theories/tests/higher_order.v
@@ -4,8 +4,9 @@ Section example.
   Context `{clangG Σ}.
 
   Definition abs_spec g E (P Q: iProp Σ) :=
-    (∃ gbody, text_interp g (Function Tvoid [] gbody) ∗
-              (∀ Φ k ks, P -∗ (Q -∗ WP (fill_ectxs void k, ks) {{ Φ }}) -∗ WP (gbody, k::ks) @ E {{ Φ }}))%I.
+    (∃ gbody, g T↦ Function Tvoid [] gbody ∗
+                (∀ Φ k ks, P -∗ (Q -∗ WP (fill_ectxs void k, ks) {{ Φ }}) -∗
+                           WP (gbody, k::ks) @ E {{ Φ }}))%I.
 
   Lemma higher_order_spec k ks E g Φ P Q:
     abs_spec g E P Q ∗ P ∗ (Q -∗ WP (fill_ectxs void k, ks) {{ Φ }})
