theories/tests/spawn.v
@@ -17,18 +17,18 @@ Section test.
 
   Lemma add_safe ks:
     is_lock N γ l R ∗
-    text_interp "release" (Function Tvoid [("x", tylock)] release) ∗
-    text_interp "acquire" (Function Tvoid [("x", tylock)] acquire)
+    "release" T↦ Function Tvoid [("x", tylock)] release ∗
+    "acquire" T↦ Function Tvoid [("x", tylock)] acquire
     ⊢ WP (add, ks) {{ _, True }}.
   Proof.
-    iIntros "(#Hlk & H1 & H2)". unfold add.
+    iIntros "(#Hlk & #? & #?)". unfold add.
     wp_unfill (Ecall _ _ _).
-    iApply acquire_spec. iFrame. iFrame "#".
+    iApply acquire_spec. iFrame "#".
     iIntros "Hlked HR".
     iDestruct "HR" as (?) "Hvx".
     wp_skip. wp_load. wp_op. wp_assign.
-    iApply (release_spec []). iFrame "Hlk".
-    iFrame. iSplitL "Hvx"; first by iExists _.
+    iApply (release_spec []). iFrame "Hlked Hlk". iFrame "#".
+    iSplitL "Hvx"; first by iExists _.
     iApply wp_value=>//.
   Qed.
 
@@ -41,21 +41,18 @@ Section test.
 
   Lemma spawn_spec ks:
     is_lock N γ l R ∗
-    text_interp "release" (Function Tvoid [("x", tylock)] release) ∗
-    text_interp "acquire" (Function Tvoid [("x", tylock)] acquire) ∗
-    text_interp "add" (Function Tvoid [] add)
+    "release" T↦ Function Tvoid [("x", tylock)] release ∗
+    "acquire" T↦ Function Tvoid [("x", tylock)] acquire ∗
+    "add" T↦ Function Tvoid [] add
     ⊢ WP (spawn, ks) {{ _, True }}.
   Proof.
-    iIntros "(#Hlk & Hf1 & Hf2 & Hf3)".
+    iIntros "(#Hlk & #? & #? & #?)".
     unfold spawn. iApply wp_seq=>//.
-    iDestruct (text_interp_dup with "Hf3") as "[Hf3 ?]".
-    iApply (wp_fork _ _ _ []); last iFrame; first done.
-    iNext. iDestruct (text_interp_dup with "Hf1") as "[Hf1 Hf1']".
-    iDestruct (text_interp_dup with "Hf2") as "[Hf2 Hf2']".
-    iSplitL "Hf1 Hf2 Hf3".
-    - wp_skip. iApply (wp_fork _ _ _ []); last iFrame; first done.
-      iNext. iSplit=>//. iApply add_safe. by iFrame.
-    - iApply add_safe. by iFrame.
+    iApply (wp_fork _ _ _ []); last iFrame "#"; first done.
+    iNext. iSplitL "".
+    - wp_skip. iApply (wp_fork _ _ _ []); last iFrame "#"; first done.
+      iNext. iSplit=>//. iApply add_safe. iFrame "#".
+    - iApply add_safe. iFrame "#".
   Qed.
 
 End test.
